Kraken/Examples/Cond.lean
@@ -1,4 +1,4 @@
-import Kraken.X64MNew
+import Kraken.X64M
 import Std.Tactic.BVDecide
 
 open Std.Internal.Do
@@ -8,7 +8,7 @@ set_option mvcgen.warning false
 set_option grind.warning false
 set_option maxHeartbeats 1000000
 
-def condProg (l : Int64) : X64MNew Unit Unit := do
+def condProg (l : Int64) : X64M Unit Unit := do
   Op.dec (.reg (.low .rax .W64))
   Op.jcc .nz l
   Op.mov (.reg (.low .rbx .W64)) (.imm (.int64 7))
